local.get

Tibi/Compiler.lean
@@ -9,12 +9,14 @@ open Wasm.Value
 inductive CompileError
 | OutOfBounds_Int64 (n : Int)
 
-def Expr.compile : Expr → Except CompileError (List Wasm.Instr)
+def Expr.compile : Expr ctx ty → Except CompileError (List Wasm.Instr)
 | .Const n =>
     if h : (-Int64.size : Int) ≤ n ∧ n < Int64.size then
-      .ok [.i64__const <| Int64.mk ⟨n, h.right, h.left⟩]
+      .ok [.i64.const <| Int64.mk ⟨n, h.right, h.left⟩]
     else
       .error <| .OutOfBounds_Int64 n
+| .Var x =>
+    .ok [.local.get x.idx]
 
 def CompileError.toString : CompileError → String
 | .OutOfBounds_Int64 n => s!"{n} is out of Int64 bounds, should be satisfied that -2{Nat.toSuperscriptString 63} ≤ n < 2{Nat.toSuperscriptString 63}"
