Tibi/Interpreter.lean
@@ -5,7 +5,7 @@ import Tibi.Util
 
 namespace Tibi
 
-def Expr.eval : (e : Expr) → {{ r | Eval e r }}
+def Expr.eval (env : Env ctx) : (e : Expr ctx ty) → {{ r | Eval env e r }}
 | .Const n =>
     if h : (-Int64.size : Int) ≤ n ∧ n < Int64.size then
       .found (.ok <| Int64.mk ⟨n, h.right, h.left⟩) <| Eval.Const h.right h.left
@@ -13,3 +13,4 @@ def Expr.eval : (e : Expr) → {{ r | Eval e r }}
       Decidable.not_and_iff_or_not_not.mp h |>.by_cases
         (fun h => .found (.error <| .OutOfBounds_Int64 n) <| Eval.ConstErr_ge h)
         (fun h => .found (.error <| .OutOfBounds_Int64 n) <| Eval.ConstErr_lt h)
+| .Var x => .found (.ok <| env.lookup x) <| Eval.Var x
