Tibi/Syntax/Expr.lean
@@ -1,10 +1,39 @@
 import Tibi.FinInt
+import Tibi.Util
 
 namespace Tibi
 
-inductive Expr
-| Const : Int → Expr
+inductive Ty where
+| int
 
-instance : ToString Expr where
-  toString
-  | .Const n => s!"<Const {n}>"
+@[reducible]
+def Ty.interp : Ty → Type
+| int => Int64
+
+def Ty.toString : Ty → String
+| int => "Int"
+
+instance : ToString Ty where
+  toString := Ty.toString
+
+inductive Locals : Fin n → Tibi.Vec Ty n → Ty → Type where
+| stop : Locals 0 (ty :: ctx) ty
+| pop  : Locals k ctx ty → Locals k.succ (u :: ctx) ty
+
+def Locals.idx : Locals n ctx ty → Fin n.succ
+| stop  => Fin.mk 0 (Fin.succ_pos _)
+| pop k => k.idx.succ
+
+instance : ToString (Locals n ctx ty) where
+  toString x := s!"${x.idx}"
+
+inductive Expr : Vec Ty n → Ty → Type where
+| Const : Int → Expr ctx .int
+| Var   : Locals i ctx ty → Expr ctx ty
+
+def Expr.toString : Expr ctx ty → String
+| Const n => s!"<Const {n}>"
+| Var x   => s!"<Var {x} @{ty}>"
+
+instance : ToString (Expr ctx ty) where
+  toString := Expr.toString
