Tibi/Typing.lean
@@ -1,4 +1,5 @@
 import Tibi.FinInt
+import Tibi.Semantics
 import Tibi.Syntax
 import Tibi.Util
 
@@ -14,12 +15,18 @@ def Typ.toString : Typ → String
 instance : ToString Typ where
   toString := Typ.toString
 
-inductive HasType : Expr → Typ → Prop
-| Int64 {n : Int} (hLt : n < Int64.size) (hGe : n ≥ -Int64.size) : HasType (.Const n) .Int64
+def Ty.toTyp : Ty → Typ
+| int => .Int64
 
-def Expr.typeCheck : (e : Expr) → {{ t | HasType e t }}
+inductive HasType (env : Env ctx) : Expr ctx ty → Typ → Prop
+| Int64 {n : Int} (hLt : n < Int64.size) (hGe : n ≥ -Int64.size) : HasType env (.Const n) .Int64
+| Var {x : Locals i ctx ty} : HasType env (.Var x) ty.toTyp
+
+def Expr.typeCheck (env : Env ctx) : (e : Expr ctx ty) → {{ t | HasType env e t }}
 | .Const n =>
     if h : -Int64.size ≤ n ∧ n < Int64.size then
       .found .Int64 <| .Int64 h.right h.left
     else
       .unknown
+| .Var _ =>
+      .found ty.toTyp .Var
