Tibi/Wasm/Semantics/Reduction.lean
@@ -9,9 +9,12 @@ open Wasm.Value
 /- # Wasm Reduction -/
 
 inductive Reduction : Configuration → Configuration → Prop
-| i32__const {i : Int32} : Reduction
-    { instrs := .i32__const i :: K, stack := s,                             store, framestate }
+| i32.const {i : Int32} : Reduction
+    { instrs := .i32.const i :: K, stack := s,                             store, framestate }
     { instrs := K,                  stack := .Value (.Num (.Int32 i)) :: s, store, framestate }
-| i64__const {i : Int64} : Reduction
-    { instrs := .i64__const i :: K, stack := s,                             store, framestate }
+| i64.const {i : Int64} : Reduction
+    { instrs := .i64.const i :: K, stack := s,                             store, framestate }
     { instrs := K,                  stack := .Value (.Num (.Int64 i)) :: s, store, framestate }
+| local.get (n : Nat) : Reduction
+    { instrs := .local.get n :: K, stack := s,                                      store, framestate }
+    { instrs := K,                  stack := .Value (framestate.locals.get! n) :: s, store, framestate }
