Tibi/Props/Compiler.lean
@@ -4,15 +4,35 @@ import Tibi.Wasm.Semantics
 
 namespace Tibi
 
-theorem Wasm.Reduction.of_has_type_of_eval_ok_of_compile_ok -- Expr.compile_ok_of_has_type_of_eval
-: {e : Expr} → HasType e _ty → Eval e (.ok v) → {_ : e.compile = .ok instrs}
+/-
+type mismatch
+  Wasm.Reduction.local__get ↑x.idx
+has type
+  Wasm.Reduction
+    { stack := ?m.4159, store := ?m.4160, framestate := ?m.4161, instrs := Wasm.Instr.local.get ↑x.idx :: ?m.4162 }
+    { stack := Wasm.StackValue.Value (?m.4161.locals.get! ↑x.idx) :: ?m.4159, store := ?m.4160, framestate := ?m.4161,
+      instrs := ?m.4162 } : Prop
+but is expected to have type
+  Wasm.Reduction
+    { stack := stack, store := store, framestate := framestate, instrs := [Wasm.Instr.local.get ↑x.idx] ++ K }
+    { stack := Wasm.StackValue.Value (Wasm.Value.Num (Wasm.Num.Int64 (Env.lookup x env))) :: stack, store := store,
+      framestate := framestate, instrs := K } : Prop
+
+theorem Wasm.Reduction.of_has_type_of_eval_ok_of_compile_ok
+: {e : Expr ctx ty} → HasType env e _ty → Eval env e (.ok v) → {_ : e.compile = .ok instrs}
 → Wasm.Reduction
     { instrs := instrs ++ K, stack,                                      store, framestate }
     { instrs := K,           stack := .Value (.Num (.Int64 v)) :: stack, store, framestate }
 | .Const n, .Int64 hLt hGe, .Const _ _, hc => by
-    have : (Expr.Const n).compile = .ok [.i64__const (Int64.mk ⟨n, hLt, hGe⟩)] := by
+    have : (Expr.Const n : Expr ctx ty).compile = .ok [.i64.const (Int64.mk ⟨n, hLt, hGe⟩)] := by
       -- dsimp [Expr.compile]
       apply dite_cond_eq_true <| eq_true <| And.intro hGe hLt
-    have : instrs = [.i64__const ⟨n, hLt, hGe⟩ ] := Except.ok.inj <| Eq.trans hc.symm this
+    have : instrs = [.i64.const ⟨n, hLt, hGe⟩] := Except.ok.inj <| Eq.trans hc.symm this
     rw [this]
-    exact .i64__const
+    exact .i64.const
+| .Var x, .Var, .Var _, hc => by
+    have : (Expr.Var x : Expr ctx ty).compile = .ok [.local.get x.idx] := rfl
+    have : instrs = [.local.get x.idx] := Except.ok.inj <| Eq.trans hc.symm this
+    rw [this]
+    exact .local.get x.idx
+-/
