Tibi/Props/Typing.lean
@@ -3,28 +3,28 @@ import Tibi.Typing
 
 namespace Tibi
 
-theorem HasType.det (h₁ : HasType e t₁) (h₂ : HasType e t₂) : t₁ = t₂ := by
+theorem HasType.det (h₁ : HasType rnv e t₁) (h₂ : HasType env e t₂) : t₁ = t₂ := by
   cases h₁ <;> cases h₂ <;> rfl
 
-theorem Expr.typeCheck_correct {e : Expr}
-: (ht : HasType e ty) → e.typeCheck = .found ty ht
+theorem Expr.typeCheck_correct {e : Expr ctx ty}
+: (ht : HasType env e t) → e.typeCheck env = .found ty.toTyp ht
 | .Int64 (n := n) hLt hGe =>
     have := eq_true <| And.intro (ge_iff_le.mp hGe) hLt
     dite_cond_eq_true this
+| .Var => rfl
 
-theorem Expr.typeCheck_complete {e : Expr}
-: e.typeCheck = .unknown → ¬ HasType e ty
+theorem Expr.typeCheck_complete {e : Expr ctx ty}
+: e.typeCheck env = .unknown → ¬ HasType env e ty.toTyp
 := by
   dsimp [Expr.typeCheck]
-  intro h (ht : HasType e ty)
+  intro h (ht : HasType env e ty.toTyp)
   match ht with
   | .Int64 hLt hGe =>
-      have := eq_true <| And.intro (ge_iff_le.mp hGe) hLt
-      have := h ▸ dite_cond_eq_true this
-      exact Maybe.noConfusion this
+      simp at h
+      exact h hGe hLt
 
-instance (e : Expr) (t : Typ) : Decidable (HasType e t) :=
-  match h : e.typeCheck with
+instance (e : Expr ctx ty) (t : Typ) : Decidable (HasType env e t) :=
+  match h : e.typeCheck env with
   | .found t' ht' =>
       if heq : t = t' then
         isTrue (heq ▸ ht')
@@ -32,8 +32,9 @@ instance (e : Expr) (t : Typ) : Decidable (HasType e t) :=
         isFalse fun ht => heq (HasType.det ht ht')
   | .unknown => isFalse (Expr.typeCheck_complete h)
 
-theorem type_safe {e : Expr}
-: HasType e t → Eval e r → ∃ v, r = .ok v
+theorem type_safe {e : Expr ctx ty}
+: HasType env e t → Eval env e r → ∃ v, r = .ok v
 | .Int64 hLt hGe, .Const ..      => ⟨Int64.mk ⟨_, hLt, hGe⟩, rfl⟩
 | .Int64 hLt _,   .ConstErr_lt h => absurd hLt h
 | .Int64 _   hGe, .ConstErr_ge h => absurd hGe h
+| .Var,           .Var x => ⟨env.lookup x, rfl⟩
