Tibi/Semantics/Eval.lean
@@ -1,0 +1,24 @@
+import Tibi.FinInt
+import Tibi.Semantics.Env
+import Tibi.Syntax
+
+namespace Tibi
+
+inductive EvalError
+| OutOfBounds_Int64 (n : Int)
+
+inductive Eval (env : Env ctx) : (Expr ctx ty) → Except EvalError Int64 → Prop
+| Const {n : Int} (hLt : n < Int64.size) (hGe : n >= -Int64.size)
+  : Eval env (.Const n) (.ok <| Int64.mk ⟨n, hLt, hGe⟩)
+| ConstErr_lt {n : Int} (h : ¬ n < Int64.size)
+  : Eval env (.Const n) (.error <| .OutOfBounds_Int64 n)
+| ConstErr_ge {n : Int} (h : ¬ n >= -Int64.size)
+  : Eval env (.Const n) (.error <| .OutOfBounds_Int64 n)
+| Var (x : Locals i ctx ty)
+  : Eval env (.Var x) (.ok (env.lookup x))
+
+def EvalError.toString : EvalError → String
+| .OutOfBounds_Int64 n => s!"{n} is out of Int64 bounds, should be satisfied that -2{Nat.toSuperscriptString 63} ≤ n < 2{Nat.toSuperscriptString 63}"
+
+instance : ToString EvalError where
+  toString := EvalError.toString
