Tibi/Util.lean
@@ -9,3 +9,9 @@ inductive Maybe (p : α → Prop)
 | found (a : α) : p a → Maybe p
 
 notation "{{ " x " | " p " }}" => Maybe (fun x => p)
+
+inductive Vec (α : Type u) : Nat → Type u
+| nil : Vec α 0
+| cons : α → Vec α n → Vec α n.succ
+
+infix:67 " :: " => Vec.cons
